cclc

coq/clc_semantics/clc_semantics.v
@@ -3,104 +3,364 @@ From Coq Require Import ssrfun Utf8 Classical.
 Require Import AutosubstSsr ARS 
   clc_context clc_ast clc_confluence clc_subtype clc_typing
   clc_weakening clc_substitution clc_inversion clc_validity
-  clc_soundness.
+  clc_soundness clc_resolution.
 
-Definition env T := seq (nat * T).
-
-Fixpoint free0 {T} (e : env T) (l : nat) : env T :=
-  match e with
-  | nil => nil
-  | (addr, m) :: e =>
-    if l == addr then e else (addr, m) :: free0 e l
-  end.
-
-Definition free {T} (e : env T) (l : nat) (t : sort) := 
-  match t with
-  | U => e
-  | L => free0 e l
-  end.
-
-Inductive open {T} : env T -> nat -> Prop :=
-| open_nil l : 
-  open nil l
-| open_cons e l addr m :
-  open e l ->
-  l <> addr ->
-  open ((addr, m) :: e) l.
-
-Inductive mapsto {T} : env T -> nat -> T -> Prop :=
-| mapsto0 e l m :
-  mapsto ((l, m) :: e) l m
-| mapsto1 e l addr m n :
-  mapsto e l m ->
-  mapsto ((addr, n) :: e) l m.
+Set Implicit Arguments.
+Unset Strict Implicit.
+Unset Printing Implicit Defensive.
 
 Inductive value : term -> Prop :=
-| value_sort s l : value (Sort s l)
-| value_pi A B s t : value (Pi A B s t)
-| value_lam A m s t : value (Lam A m s t)
-| value_unit : value Unit
-| value_it : value It
-| value_sigma A B s r t : value (Sigma A B s r t)
-| value_pair lm ln t : value (Pair (Ptr lm) (Ptr ln) t).
+| value_sort s l :
+  value (Sort s l)
+| value_pi A B s t :
+  value (Pi A B s t)
+| value_lam A m s t :
+  value (Lam A m s t)
+| value_unit :
+  value Unit
+| value_it :
+  value It
+| value_sigma A B s r t :
+  value (Sigma A B s r t)
+| value_pair m n t :
+  value m ->
+  value n ->
+  value (Pair m n t).
 
-Inductive venv : env term -> Prop :=
-| venv_nil : venv nil
-| venv_cons Θ l v : venv Θ -> value v -> venv ((l, v) :: Θ).
+Inductive cbv_step : term -> term -> Prop :=
+| cbv_appL m m' n :
+  cbv_step m m' ->
+  cbv_step (App m n) (App m' n)
+| cbv_appR m n n' :
+  value m ->
+  cbv_step (App m n) (App m n')
+| cbv_beta A m n s t :
+  value n ->
+  cbv_step (App (Lam A m s t) n) m.[n/]
+| cbv_pairL m m' n t :
+  cbv_step m m' ->
+  cbv_step (Pair m n t) (Pair m' n t)
+| cbv_pairR m n n' t :
+  value m ->
+  cbv_step n n' ->
+  cbv_step (Pair m n t) (Pair m n' t)
+| cbv_letin1 m m' n :
+  cbv_step m m' ->
+  cbv_step (LetIn1 m n) (LetIn1 m' n)
+| cbv_iota1 n :
+  cbv_step (LetIn1 It n) n
+| cbv_letin2 m m' n :
+  cbv_step m m' ->
+  cbv_step (LetIn2 m n) (LetIn2 m' n)
+| cbv_iota2 m1 m2 n t :
+  cbv_step (LetIn2 (Pair m1 m2 t) n) n.[m2,m1/].
 
-Reserved Notation "Θ ;; m => Θ' ;; n" 
-  (at level 80, m, Θ', n at next level).
-
-Inductive eval : env term -> term -> env term -> term -> Prop :=
+Inductive eval : context term -> term -> context term -> term -> Prop :=
 | eval_sort Θ s i l :
-  open Θ l ->
-  Θ ;; Sort s i => (l, Sort s i) :: Θ ;; Ptr l
+  l = length Θ ->
+  eval Θ (Sort s i) (Sort s i :U Θ) (Ptr l)
 | eval_pi Θ A B s t l :
-  open Θ l ->
-  Θ ;; Pi A B s t => (l, Pi A B s t) :: Θ ;; Ptr l
+  l = length Θ ->
+  eval Θ (Pi A B s t) (Pi A B s t :U Θ) (Ptr l)
 | eval_lam Θ A m s t l :
-  open Θ l ->
-  Θ ;; Lam A m s t => (l, Lam A m s t) :: Θ ;; Ptr l
+  l = length Θ ->
+  eval Θ (Lam A m s t) (Lam A m s t :{t} Θ) (Ptr l)
 | eval_appL Θ Θ' m m' n :
-  Θ ;; m => Θ' ;; m' ->
-  Θ ;; App m n => Θ' ;; App m' n
+  eval Θ m Θ' m' ->
+  eval Θ (App m n) Θ' (App m' n)
 | eval_appR Θ Θ' l n n' :
-  Θ ;; n => Θ' ;; n' ->
-  Θ ;; App (Ptr l) n => Θ' ;; App (Ptr l) n'
+  eval Θ n Θ' n' ->
+  eval Θ (App (Ptr l) n) Θ' (App (Ptr l) n')
 | eval_beta Θ Θ' lf la A m s t :
-  Θ' = free Θ lf t ->
-  mapsto Θ lf (Lam A m s t) ->
-  Θ ;; App (Ptr lf) (Ptr la) => Θ' ;; m.[Ptr la/]
+  free Θ lf (Lam A m s t) Θ' ->
+  eval Θ (App (Ptr lf) (Ptr la)) Θ' m.[Ptr la/]
 | eval_unit Θ l :
-  open Θ l ->
-  Θ ;; Unit => (l, Unit) :: Θ ;; Ptr l
+  l = length Θ ->
+  eval Θ Unit (Unit :U Θ) (Ptr l)
 | eval_it Θ l :
-  open Θ l ->
-  Θ ;; It => (l, It) :: Θ ;; Ptr l
+  l = length Θ ->
+  eval Θ It (It :U Θ) (Ptr l)
 | eval_sigma Θ A B s r t l :
-  open Θ l ->
-  Θ ;; Sigma A B s r t => (l, Sigma A B s r t) :: Θ ;; Ptr l
+  l = length Θ ->
+  eval Θ (Sigma A B s r t) (Sigma A B s r t :U Θ) (Ptr l)
 | eval_pairL Θ Θ' m m' n t :
-  Θ ;; m => Θ' ;; m' ->
-  Θ ;; Pair m n t => Θ' ;; Pair m' n t
+  eval Θ m Θ' m' ->
+  eval Θ (Pair m n t) Θ' (Pair m' n t)
 | eval_pairR Θ Θ' l n n' t :
-  Θ ;; n => Θ' ;; n' ->
-  Θ ;; Pair (Ptr l) n t => Θ' ;; Pair (Ptr l) n' t
+  eval Θ n Θ' n' ->
+  eval Θ (Pair (Ptr l) n t) Θ' (Pair (Ptr l) n' t)
 | eval_pairV Θ l lm ln t :
-  open Θ l ->
-  Θ ;; Pair (Ptr lm) (Ptr ln) t => 
-  (l, Pair (Ptr lm) (Ptr ln) t) :: Θ ;; Ptr l
+  l = length Θ ->
+  eval Θ (Pair (Ptr lm) (Ptr ln) t)
+         ((Pair (Ptr lm) (Ptr ln) t) :{t} Θ) (Ptr l)
 | eval_letin1 Θ Θ' m m' n :
-  Θ ;; m => Θ' ;; m' ->
-  Θ ;; LetIn1 m n => Θ' ;; LetIn1 m' n
-| eval_iota1 Θ l n :
-  mapsto Θ l It ->
-  Θ ;; LetIn1 (Ptr l) n => Θ ;; n
+  eval Θ m Θ' m' ->
+  eval Θ (LetIn1 m n) Θ' (LetIn1 m' n)
+| eval_iota1 Θ Θ' l n :
+  free Θ l It Θ' ->
+  eval Θ (LetIn1 (Ptr l) n) Θ' n
 | eval_iota2 Θ Θ' lm ln l n t :
-  Θ' = free Θ l t ->
-  mapsto Θ l (Pair (Ptr lm) (Ptr ln) t) ->
-  Θ ;; LetIn2 (Ptr l) n => Θ' ;; n.[Ptr ln,Ptr ln/]
-where "Θ ;; m => Θ' ;; n" := (eval Θ m Θ' n).
+  free Θ l (Pair (Ptr lm) (Ptr ln) t) Θ' ->
+  eval Θ (LetIn2 (Ptr l) n) Θ' n.[Ptr ln,Ptr ln/].
 
-Theorem progress m A Θ :
-  nil ⊢ m : A -> 
+(* Lemma eval_red Θ1 Θ1' Θ2 Θ2' Θ Θ' m m' n n' :
+  resolve Θ1 m n -> Θ1 ∘ Θ2 => Θ -> eval Θ m Θ' m' ->
+  resolve Θ1' m' n' -> pad Θ2 Θ2' -> Θ1' ∘ Θ2' => Θ' ->
+  n ~>* n'.
+Proof.
+  move=>rs. elim: rs Θ1' Θ2 Θ2' Θ Θ' m' n'=>{Θ1 m n}.
+  move=>Θ x k Θ1' Θ2 Θ2' Θx Θ' m' n' mrg1 ev rs pd mrg2.
+  { inv ev. }
+  move=>Θ s l k Θ1' Θ2 Θ2' Θx Θ' m' n' mrg1 ev rs pd mrg2.
+  { inv ev. inv mrg2.
+    have[e1 e2]:=merge_length H2.
+    rewrite<-e1 in rs.
+    inv rs.
+    move/free_inv in H0; subst.
+    inv H3.
+    eauto. }
+  move=>Θ A A' B B' s t k rsA ihA rsB ihB
+   Θ1' Θ2 Θ2' Θx Θ' m' n'  mrg1 ev rs pd mrg2.
+  { inv ev. inv mrg2. inv pd.
+    have[e1 e2]:=merge_length H2.
+    rewrite<-e1 in rs.
+    inv rs.
+    have[e3 e4]:=free_inv H0; subst.
+    inv H3.
+    eauto.
+    apply: red_pi.
+    apply: ihA; eauto.
+    apply: mrg1.
+    eauto. }
+
+Admitted. *)
+
+
+Lemma eval_split Θ1 Θ2 Θ Θ' Γ m n m' A :
+  ok Γ -> well_resolved Θ1 Γ m n A ->  
+  Θ1 ∘ Θ2 => Θ -> eval Θ m Θ' m' ->
+  exists Θ1' Θ2' n', 
+    well_resolved Θ1' Γ m' n' A /\ 
+    pad Θ2 Θ2' /\ Θ1' ∘ Θ2' => Θ' /\ n ~>* n'.
+Proof with eauto using 
+  clc_type, resolve, resolve_wkU, resolve_wkN, free, pad, merge.
+  move=>wf [rm tyn].
+  elim: tyn wf Θ1 Θ2 Θ Θ' m m' rm=>{Γ n A}.
+  move=>Γ s l k wf Θ1 Θ2 Θ Θ' m m' rsm mrg ev.
+  { inv rsm; inv ev.
+    exists ((s @ l) :U Θ1).
+    exists ((s @ l) :U Θ2).
+    exists (s @ l).
+    repeat split...
+    move:mrg=>/merge_length[<-_].
+    repeat split... }
+  move=>Γ A B s r t i k tyA ihA tyB ihB wf Θ1 Θ2 Θ Θ' m m' rsm mrg ev.
+  { inv rsm; inv ev.
+    exists ((Pi A0 B0 s t) :U Θ1).
+    exists ((Pi A0 B0 s t) :U Θ2).
+    exists (Pi A B s t).
+    repeat split...
+    move:mrg=>/merge_length[<-_].
+    repeat split... }
+  move=>Γ x A s hs wf Θ1 Θ2 Θ Θ' m m' rsm mrg ev.
+  { inv rsm; inv ev. }
+  move=>Γ A B m s t i k tyP ihP tym ihm wf Θ1 Θ2 Θ Θx n m' rsL mrg ev.
+  { inv rsL; inv ev.
+    have[<-_]:=merge_length mrg.
+    destruct t.
+    { exists ((Lam A0 m0 s U) :U Θ1).
+      exists ((Lam A0 m0 s U) :U Θ2).
+      exists (Lam A m s U).
+      repeat split... }
+    { exists ((Lam A0 m0 s L) :L Θ1).
+      exists (_: Θ2).
+      exists (Lam A m s L).
+      repeat split... } }
+  move=>Γ1 Γ2 Γ A B m n s t k mrg1 tym ihm tyn ihn
+    wf Θ1 Θ2 Θ Θ' x x' rx mrg2 ev.
+  { have[wf1 wf2]:=merge_context_ok_inv mrg1 wf.
+    have[r[l tyP]]:= validity wf1 tym.
+    have[r0[l0[tyA tyB]]]:= pi_inv _ _ _ _ _ _ tyP.
+    inv rx; inv ev.
+    { have[Θx[mrg3 mrg4]]:=merge_splitR mrg2 H1.
+      have[Θx1[Θx2[mx[wr[pd[mrgx rx]]]]]]:=
+        ihm wf1 _ _ _ _ _ _ H4 mrg4 H7.
+      have[Θ3p[Θ2p[pd1[pd2 mrp]]]]:=pad_merge pd mrg3.
+      have[Θy[mrp1 mrp2]]:=merge_splitL (merge_sym mrgx) mrp.
+      move:wr=>[rx1 tyx].
+      exists Θy. exists Θ2p.
+      exists (App mx n).
+      repeat split...
+      econstructor. exact: (merge_sym mrp1).
+      exact: rx1. apply: resolve_pad...
+      apply: red_app... }
+    { have[Θx[mrg3 mrg4]]:=merge_splitL mrg2 H1.
+      have{ihn}[Θx1[Θx2[nx[wr[pd[mrgx rx]]]]]]:=
+        ihn wf2 _ _ _ _ _ _ H5 (merge_sym mrg4) H7.
+      have[Θ3p[Θ2p[pd1[pd2 mrp]]]]:=pad_merge pd mrg3.
+      have[Θy[mrp1 mrp2]]:=merge_splitL (merge_sym mrgx) mrp.
+      move:wr=>[rx1 tyx].
+      exists Θy. exists Θ2p.
+      exists (App m nx).
+      repeat split...
+      econstructor. exact: mrp1.
+      apply: resolve_pad... exact: rx1.
+      have[e1[e2 e3]]:=merge_re_re mrg1.
+      destruct s.
+      { apply: clc_conv.
+        apply: conv_sub.
+        apply: conv_beta.
+        apply: conv_sym.
+        apply: star_conv.
+        apply: rx.
+        apply: clc_app...
+        have mrgs:[Γ1] ∘ Γ2 => Γ2.
+        rewrite e1. apply: merge_reL.
+        have h:=substitution tyB k mrgs tyn.
+        rewrite<-e3.
+        rewrite<-pure_re... }
+      { apply: clc_conv.
+        apply: conv_sub.
+        apply: conv_beta.
+        apply: conv_sym.
+        apply: star_conv.
+        apply: rx.
+        apply: clc_app...
+        have h:=substitutionN tyB tyn.
+        rewrite e2 in h... }
+      apply: red_app... } 
+    { move=>{ihm ihn}.
+      inv H4.
+
+    }
+  }
+
+
+  (* move=>Γ s l k wf Θ1 Θ2 Θ Θ' m m' A rsm rsA mrg ev.
+  { inv rsm; inv ev.
+    exists ((s @ l) :U Θ1).
+    exists ((s @ l) :U Θ2).
+    repeat split...
+    move:mrg=>/merge_length[<-_].
+    exists (s @ l). exists (U @ l.+1).
+    repeat split... }
+  move=>Γ A B s r t i k tyA ihA tyB ihB wf Θ1 Θ2 Θ Θ' m m' C
+    rsm rsC mrg ev.
+  { inv rsm; inv ev.
+    exists ((Pi A0 B0 s t) :U Θ1).
+    exists ((Pi A0 B0 s t) :U Θ2).
+    repeat split...
+    move:mrg=>/merge_length[<-_].
+    exists (Pi A B s t). exists (t @ i).
+    repeat split... }
+  move=>Γ x A s hs wf Θ1 Θ2 Θ Θ' m m' C rsm rsC mrg ev.
+  { inv rsm; inv ev. }
+  move=>Γ A B m s t i k tyP ihP tym ihm wf Θ1 Θ2 Θ Θx n m' C
+    rsL rsC mrg ev.
+  { inv rsL; inv ev.
+    have[<-_]:=merge_length mrg.
+    destruct t.
+    { exists ((Lam A0 m0 s U) :U Θ1).
+      exists ((Lam A0 m0 s U) :U Θ2).
+      repeat split...
+      exists (Lam A m s U). exists (Pi A B s U).
+      repeat split... }
+    { exists ((Lam A0 m0 s L) :L Θ1).
+      exists (_: Θ2).
+      repeat split...
+      exists (Lam A m s L). exists (Pi A B s L).
+      repeat split... } }
+  move=>Γ1 Γ2 Γ A B m n s t k mrg1 tym ihm tyn ihn
+    wf Θ1 Θ2 Θ Θ' x x' C rx rC mrg2 ev.
+  { have[wf1 wf2]:=merge_context_ok_inv mrg1 wf.
+    have[r[l tyP]]:= validity wf1 tym.
+    have[r0[l0[tyA tyB]]]:= pi_inv _ _ _ _ _ _ tyP.
+    inv rx; inv ev.
+    { have rP:=resolve_type_refl Θ0 tyP.
+      have[Θx[mrg3 mrg4]]:=merge_splitR mrg2 H1.
+      have{ihm}[Θx1[Θx2[wr[pd mrgx]]]]:=
+        ihm wf1 _ _ _ _ _ _ _ H4 rP mrg4 H7.
+      have[Θ3p[Θ2p[pd1[pd2 mrp]]]]:=pad_merge pd mrg3.
+      have[Θy[mrp1 mrp2]]:=merge_splitL (merge_sym mrgx) mrp.
+      exists Θy. exists Θ2p.
+      repeat split...
+      move:wr=>[mx[tyPx[rx1[rx2 tyx]]]].
+      exists (App mx n). exists (B.[n/]).
+      repeat split.
+      econstructor. exact: (merge_sym mrp1).
+      exact: rx1. apply: resolve_pad...
+      have[_[<-_]]:=merge_re_re mrp1.
+      apply: resolve_pad.
+      apply: pad_re...
+      have[_[_->]]:=merge_re_re H1...
+      have e:=resolve_type_id tyP rx2; subst.
+      apply: clc_app... }
+    { have rA:=resolve_type_refl Θ3 tyA.
+      have[Θx[mrg3 mrg4]]:=merge_splitL mrg2 H1.
+      have{ihn}[Θx1[Θx2[wr[pd mrgx]]]]:=
+        ihn wf2 _ _ _ _ _ _ _ H5 rA (merge_sym mrg4) H7.
+      have[Θ3p[Θ2p[pd1[pd2 mrp]]]]:=pad_merge pd mrg3.
+      have[Θy[mrp1 mrp2]]:=merge_splitL (merge_sym mrgx) mrp.
+      exists Θy. exists Θ2p.
+      repeat split...
+      move:wr=>[nx[tyPx[rx1[rx2 tyx]]]].
+      exists (App m nx). exists (B.[nx/]).
+      repeat split.
+      econstructor. exact: mrp1.
+      apply: resolve_pad... exact: rx1.
+      have[_[<-_]]:=merge_re_re mrp1.
+      apply: resolve_pad.
+      apply: pad_re...
+      have[_[->_]]:=merge_re_re H1...
+      have:=eval_red _.
+      admit.
+      have e:=resolve_type_id tyA rx2; subst.
+      apply: clc_app... }
+
+  }
+Admitted. *)
+
+Lemma well_resolved_eval Θ Θ' Γ m m' A :
+  well_resolved Θ Γ m A -> eval Θ m Θ' m' -> well_resolved Θ' Γ m' A.
+Proof with eauto using 
+  clc_type, resolve, resolve_wkU, resolve_wkN, free.
+  move=>[n[B[rm[rA tyn]]]].
+  elim: tyn Θ Θ' m m' A rm rA=>{Γ n B}.
+  move=>Γ s l k Θ Θ' m m' A rsm rsA ev.
+  { inv rsm. inv ev.
+    exists (s @ l). exists (U @ l.+1).
+    repeat split...
+    inv ev. }
+  move=>Γ A B s r t i k tyA ihA tyB ihB Θ Θ' m m' C rs1 rs2 ev.
+  { inv rs1. inv ev.
+    exists (Pi A B s t). exists (t @ i).
+    repeat split...
+    inv ev. }
+  move=>Γ x A s hs Θ Θ' m m' C rs1 rs2 ev.
+  { inv rs1. inv ev. inv ev. }
+  move=>Γ A B m s t i k tyP ihP tym ihm Θ Θ' rs n C rs1 rs2 ev.
+  { inv rs1. inv ev.
+    exists (Lam A m s t). exists (Pi A B s t).
+    destruct t; repeat split...  
+    inv ev. }
+  move=>Γ1 Γ2 Γ A B m n s t k mrg tym ihm tyn ihn 
+    Θ Θ' n' m' C rs1 rs2 ev.
+  { inv rs1. inv ev.
+    {
+      (* { have[G1[G2[mx[rs'[pd mrg']]]]]:= *)
+      have wr:well_resolved Θ1 Γ1 m0 (Pi A B s t).
+      exists m. exists (Pi A B s t).
+      repeat split...
+      admit.
+      have[G1[G2[[mx[X[rx1[rx2 tyx]]]][pd mrg']]]]:=eval_split H7 wr H1.
+      exists (App mx n). exists (B.[n/]).
+      repeat split...
+      econstructor...
+      exact rx1.
+
+    }
+    admit.
+    inv ev.
+
+  }
+
